Add remove.

Practical_Foundation_of_Programming_Languages/PLT.v
@@ -1,6 +1,6 @@
 Set Implicit Arguments.
 
-Require Import List Program.
+Require Import List Program Permutation.
 
 Definition set T := T -> Prop.
 
@@ -15,26 +15,109 @@ Inductive ihlist { F : Type -> Type } : list Type -> Type :=
 | ihcons : forall T L (f : F T), ihlist L -> ihlist (T :: L).
 
 Implicit Arguments ihlist[].
-
-Definition operator (S : Type) := list Type.
-Definition variable (S : Type) := unit.
+Implicit Arguments ihcons[T L F].
 
 Inductive Pos A : A -> list A -> Type :=
 | Pos_fst : forall a l, Pos a (a :: l)
 | Pos_skip : forall a a' l, Pos a' l -> Pos a' (a :: l).
 
-Inductive AXs
-  { S : set Type }
-    { Os : forall s, contain S s -> list (operator s) }
-    { Xs : forall s, contain S s -> list (variable s) } : Type -> Type :=
-| XAXs : forall s (c : contain S s)(va : variable s), Pos va (Xs s c) -> AXs s
-| OAXs : forall s (c : contain S s)(op : operator s), Pos op (Os s c) -> 
-    ihlist (fun s' => AXs s') op -> AXs s.
+Definition remove T (t : T) (l : list T) (P : Pos t l) :
+  { l' : list T | Permutation (t :: l') l }.
+  induction P.
+  exists l.
+  trivial.
+  destruct IHP.
+  exists (a :: x).
+  symmetry.
+  eapply (@perm_trans _ _ (a :: a' :: x)).
+  auto with *.
+  constructor.
+Defined.
 
-Implicit Arguments AXs[].
-Implicit Arguments OAXs[s c op S Os Xs].
-Implicit Arguments XAXs[s c va S Os Xs].
-Implicit Arguments ihcons[T L F].
+Inductive ihlist_forall (F : Type -> Type) { P : forall T, F T -> Type } : 
+  forall L, ihlist F L -> Type :=
+| Forall_ihnil : ihlist_forall ihnil
+| Forall_ihcons : forall (l : list Type)(L : ihlist F l)(T : Type)(t : F T), 
+    P T t -> ihlist_forall L -> ihlist_forall (ihcons t L).
+
+Implicit Arguments ihlist_forall[F].
+
+Section AST.
+  Variable S : set Type.
+  Definition operator_inner { s : Type } (c : contain S s) := list Type.
+  Variable Os : forall s (c : contain S s), list (operator_inner c).
+    (*variable is just operator with arity nil*)
+  Inductive operator { s : Type } (c : contain S s) := 
+  | op : forall o : operator_inner c, Pos o (Os c) -> operator c.
+  Definition get_arity s (c : contain S s) (ope : operator c) : list Type := 
+    match ope with op l _ => l end.
+  Inductive AXs : Type -> Type :=
+  | OAXs : forall s (c : contain S s)(op : operator c), 
+      ihlist (fun s' => AXs s') (get_arity op) -> AXs s.
+  Fixpoint AST_rect (P : forall T, AXs T -> Type)
+  (FO : forall s (c : contain S s)(op : operator c)
+    (l : ihlist (fun s' => AXs s') (get_arity op)), 
+      @ihlist_forall _ (fun t ax => P t ax) (get_arity op) l -> P s (OAXs op l))
+        T (AX : AXs T) : P T AX.
+    destruct AX.
+    apply FO.
+    induction i;
+    constructor;
+    try apply AST_rect;
+    trivial.
+  Defined.
+  Fixpoint AST_size T (ast : AXs T) : nat :=
+    match ast with
+    | OAXs _ _ _ il => 1 +
+        ((fix ilind t (l : ihlist _ t) : nat := 
+          match l with
+          | ihnil => 0
+          | ihcons _ _ a l' => AST_size a + ilind _ l'
+          end) _ il)
+    end.
+  Theorem ast_size : forall T (ast : AXs T), { n | n = AST_size ast }.
+    intros.
+    refine (@AST_rect (fun _ ast' => {n : nat | n = AST_size ast'}) _ T ast);
+    intros;
+    simpl in *.
+    induction X.
+    eauto.
+    destruct p, IHX.
+    exists (x + x0).
+    subst.
+    auto.
+  Defined.
+  Variable sdec : forall { s s' : Type } (c : contain S s)(c' : contain S s'),
+    { s = s' } + { s <> s' }.
+  Definition adjoin { s : Type } (c : contain S s) (v : operator_inner c) :
+    forall s', contain S s' ->
+      { ls : list (operator_inner c) | 
+        (s = s' -> ls = v :: (Os c)) /\
+        (s' <> s -> ls = Os c) }.
+    intros.
+    destruct (sdec c H).
+    subst.
+    eauto with *.
+    exists (Os c).
+    intuition.
+  Defined.
+  Check list_eq_dec.
+  Definition remove { s : Type } (c : contain S s) (v : operator_inner c) :
+    forall s', contain S s' ->
+      { ls : list (operator_inner c) |
+        ( s = s' -> Permutation (v :: ls) (Os c)) /\
+        (s' <> s -> ls = Os c) }.
+    intros.
+    destruct (sdec c H).
+    subst.
+    remember (Os c).
+    admit.
+    exists (Os c).
+    intuition.
+  Defined.
+End AST.
+
+Extraction ast_size. (*Testing if AST_rect is useful*)(*should not be defined with AST_size*)
 
 Definition subst { S S' } (s : S)(Heq : S ~= S') : {s' : S' | s ~= s' }.
   subst.
@@ -48,84 +131,4 @@ Theorem subst_eq : forall S (eq : S ~= S)(s : S), JMeq s (proj1_sig(subst s eq))
   trivial.
 Qed.
 
-Definition adjoin { S : set Type } (Xs : forall s, contain S s -> list (variable s))
-  { s : Type } { sdec : forall t, { s = t } + { s <> t } } (c : contain S s) (v : variable s) : 
-    forall s' (c' : contain S s'),
-      { ls : list (variable s') | 
-          (forall (eq : s = s'), ls = v :: (Xs _ c)) /\
-          (s' <> s -> ls = Xs _ c') }.
-  intros.
-  destruct (sdec s').
-  subst.
-  exists (v :: (Xs _ c)).
-  intuition.
-  exists (Xs s' c').
-  intuition.
-Defined.
-
-Inductive ihlist_forall (F : Type -> Type) { P : forall T, F T -> Type } : 
-  forall L, ihlist F L -> Type :=
-| Forall_ihnil : ihlist_forall ihnil
-| Forall_ihcons : forall (l : list Type)(L : ihlist F l)(T : Type)(t : F T), 
-    P T t -> ihlist_forall L -> ihlist_forall (ihcons t L).
-
-Implicit Arguments ihlist_forall[F].
-
-Fixpoint AST_rect S Os Xs (P : forall T, AXs S Os Xs T -> Type)
-  (FX : forall s (c : contain S s)(s' : variable s)(i : Pos s' (Xs s c)), P s (XAXs i))
-  (FO : forall s (c : contain S s)(op : operator s)(i : Pos op (Os s c))
-    (l : ihlist (fun s' => AXs S Os Xs s') op), 
-      ihlist_forall (fun t ax => P t ax) op l -> P s (OAXs i l))
-  T (AX : AXs S Os Xs T) : P T AX.
-  destruct AX;
-  trivial.
-  apply FO.
-  clear p.
-  induction i;
-  constructor;
-  try apply AST_rect;
-  trivial.
-Defined.
-
-Fixpoint AST_size S Os Xs T (ast : AXs S Os Xs T) : nat :=
-  match ast with
-  | XAXs _ _ _ _ => 1
-  | OAXs _ _ _ _ il => 1 +
-      ((fix ilind t (l : ihlist _ t) : nat := 
-        match l with
-        | ihnil => 0
-        | ihcons _ _ a l' => AST_size a + ilind _ l'
-        end) _ il)
-  end.
-
-Theorem ast_size : forall S Os Xs T (ast : AXs S Os Xs T), { n | n = AST_size ast }.
-  intros.
-  refine (@AST_rect S Os Xs (fun _ ast' => {n : nat | n = AST_size ast'}) _ _ T ast);
-  intros;
-  simpl in *.
-  eauto.
-  clear i.
-  induction X.
-  eauto.
-  destruct p, IHX.
-  exists (x + x0).
-  subst.
-  auto.
-Defined.
-
-Extraction ast_size. (*Testing if AST_rect is useful*)
-
-Inductive subeq : forall S Xs Os s s'(x : variable s)(c : contain S s)(a : AXs S Os (adjoin Xs _ x _ c) Os s')(b : AXs S Xs Os s'), Prop :=.
-
-Variables are given meaning by substitution. If x is a variable of sort s, a ∈ A[X , x ] s 0 ,
-and b ∈ A[X ] s , then [ b/x ] a ∈ A[X ] s 0 is defined to be the result of substituting b for
-every occurrence of x in a. The ast a is called the target, and x is called the subject, of the
-substitution. Substitution is defined by the following equations:
-1. [ b/x ] x = b and [ b/x ] y = y if x 6 = y.
-For example, we may check that
-ew
-2. [ b/x ] o(a 1 ; . . . ;a n ) = o( [ b/x ] a 1 ; . . . ; [ b/x ] a n ).
-[ num[2]/x ] plus(x; num[3]) = plus(num[2]; num[3]).
-We may prove by structural induction that substitution on ast’s is well-defined.
-Theorem 1.1. If a ∈ A[X , x ] , then for every b ∈ A[X ] there exists a unique c ∈ A[X ] such that
-[ b/x ] a = c
+Definition remove_op { S : set Type } { s : Type } (c : contain S s)(o : operator_inner _ c) := 1.
